Tests/DTLC/TypSpec.lean
@@ -23,28 +23,5 @@ def apply1stOn2ndFn : TypAST :=
 
 end Typ
 
--- namespace Typing
-
--- example : TrmClosed.typing Trm.false 2 Typ.false := by
---   simp [TrmClosed.typing, Trm.false, Typ.false]
-
--- example : TrmClosed.typing Trm.true 2 Typ.true := by
---   simp [TrmClosed.typing, Trm.true, Typ.true]
-
--- example : TrmClosed.typing Trm.idFn 3 Typ.idFn := by
---   simp [TrmClosed.typing, Trm.idFn, Typ.idFn]
-
--- example : TrmClosed.typing Trm.get1st 4 Typ.get1st := by
---   simp [TrmClosed.typing, Trm.get1st, Typ.get1st]
-
--- example : TrmClosed.typing Trm.get2nd 4 Typ.get2nd := by
---   simp [TrmClosed.typing, Trm.get2nd, Typ.get2nd]
-
--- example : ¬ TrmClosed.typing Trm.apply1stOn2ndFnOnTuple 6 Typ.apply1stOn2ndFnOnTuple := by
---   simp [TrmClosed.typing, Trm.apply1stOn2ndFnOnTuple, Trm.apply1stOn2ndFn, Trm.idFn,
---     Trm.false,
---     Typ.apply1stOn2ndFnOnTuple]
-
--- end Typing
 
 end Sanity
