Tests/DTLC/scratch.lean
@@ -1,5 +1,0 @@
-
-structure TT (v : Nat) : Type where
-
-
-example : Type := (v: Nat) -> TT v
